Verification of receive messages and check channels

examples/scheduler/include/read_specs.h
@@ -4,21 +4,23 @@
 
 //@rc::context `{!PacketArrivals}
 
-//@rc::inlined
-//@Definition read_update_log (t : nat) (l : list LogEntry) (fd : FD) : list LogEntry := l ++ (from_option (λ ID, [read_from_socket ID t]) [] (get_head_ID_option t l fd)).
-//@rc::end
+// This specification assumes that `__builtin_errno` returns a newly allocated pointer on each call (due to the &own in the returns). This is not very realistic, but it does not influence the verification much.
+// TODO: make this specification more realistic
+[[rc::parameters("n : Z")]]
+[[rc::requires("[is_errno n]")]]
+[[rc::returns("&own<n @ int<i32>>")]]
+[[rc::ensures("[is_errno n]")]]
+extern int *__builtin_errno(void);
 
-[[rc::parameters("data : {list Z}", "fd : Z", "l : loc", "log : {list LogEntry}","t1 : nat")]]
-[[rc::exists("t2 : nat")]]
+[[rc::parameters("data : {list Z}", "fd : Z", "l : loc", "t1 : nat", "errno : Z")]]
 [[rc::args("fd @ int<i32>", "l @ &own<{uninit (mk_array_layout u8 (Z.to_nat max_msg_len))}>", "max_msg_len @ int<u64>")]]
-[[rc::returns("{if (bool_decide (is_Some (get_head_ID_option t1 log fd))) then max_msg_len else -1} @ int<i64>")]]
-// read requires the current log and the current time
-[[rc::requires("[curr_time t1]")]]
-[[rc::requires("[curr_log log]")]]
-//the timing and the log is updated
-[[rc::ensures("[curr_time t2]")]]
-[[rc::ensures("[curr_log (read_update_log t2 log fd)]")]]
-[[rc::ensures("{t2 = t1}")]]
-[[rc::ensures("own l : array_p<u8, {get_packet_data_option (get_head_ID_option t1 log fd) `at_type` int(u8)},"
-	      "{Z.to_nat max_msg_len}>")]]
+[[rc::requires("[is_errno errno]")]]
+[[rc::requires("[curr_read_index t1]")]]
+[[rc::ensures("[curr_read_index (t1 + 1%nat)]")]]
+[[rc::exists("n : Z", "pckt : packet_ID")]]
+[[rc::returns("{if (bool_decide $ is_Some $ (packet_arrivals fd t1)) then length (get_packet_data pckt) else -1} @ int<i64>")]]
+[[rc::ensures("own l : array_p<u8, {get_packet_data pckt `at_type` int(u8)}, {Z.to_nat max_msg_len}>")]]
+[[rc::ensures("[is_errno n]")]]
+[[rc::ensures("{if  (bool_decide $ is_Some $ (packet_arrivals fd t1)) then True else n = EWOULDBLOCK}")]]
+[[rc::ensures("{pckt = {|fd := fd; read_index := t1|}}")]]
 ssize_t read(int fd, void* data, size_t msg_len);
