examples/scheduler/src/fdsched.c
@@ -48,7 +48,7 @@ void fds_init(struct fd_scheduler* fds) {
 		   "array_p<{layout_of struct_callback}, {replicate i 0%nat `at_type` callback_t}, {Z.to_nat num_msg_types}>,"
 		   "uninit<{mk_array_layout struct_message_queue (Z.to_nat num_priorities)}>,"
 		   "{replicate (Z.to_nat num_priorities) false} @ prio_bitmap_t>>>")]]
-    [[rc::constraints("{i <= num_msg_types}")]]
+    [[rc::constraints("{i ≤ num_msg_types}")]]
   for(int typ = 0; typ < NUM_MESSAGE_TYPES; typ += 1) {
     fds->sched.callbacks[typ] = (struct callback) {0, nop_callback};
   }
@@ -62,7 +62,7 @@ void fds_init(struct fd_scheduler* fds) {
             "array<{layout_of struct_callback}, {replicate (Z.to_nat num_msg_types) 0%nat `at_type` callback_t}>,"
             "array_p<struct_message_queue, {replicate priority (@nil message_data) `at_type`  message_queue}, {Z.to_nat num_priorities}>,"
             "{replicate (Z.to_nat num_priorities) false} @ prio_bitmap_t >>>")]]
-    [[rc::constraints("{priority <= num_priorities}")]]
+    [[rc::constraints("{priority ≤ num_priorities}")]]
   for(int prio = 0; prio < NUM_PRIORITIES; prio += 1) {
     fds->sched.pending[prio] = (struct message_queue) {NULL, NULL};
     fds->sched.pending[prio].last = &fds->sched.pending[prio].first;
@@ -104,30 +104,25 @@ void fds_set_callback(struct fd_scheduler* fds,
   fds->sched.callbacks[type] = (struct callback) {prio, f};
 }
 
-[[rc::parameters("fd_state : fd_sched", "p1 : loc","fd : Z", "l : {list LogEntry}","t1 : nat")]]
+[[rc::parameters("fd_state : fd_sched", "p1 : loc","fd : Z","t1 : nat", "errno : Z")]]
 [[rc::args("p1 @ &own<fd_state @ fd_t>", "fd @ int<i32>")]]
-[[rc::exists("t2 : nat")]]
-[[rc::returns("{let pending := get_pending_packets_from_given_fd t1 l fd in"
-	      "(if decide (pending = []) then -1 else 0)} @ int<i32>")]]
-//requires the time and the current log
-[[rc::requires("[curr_time t1]")]]
-[[rc::requires("[curr_log l]")]]
-//the log is only updated by read and time is also only incremented by read
-[[rc::ensures("[curr_time t2]")]]
-[[rc::ensures("{t2 = t1}")]]
-[[rc::ensures("[curr_log (read_update_log t1 l fd)]")]]
-//the scheduler state is updated to include the message (if any) returned by read
-[[rc::ensures("own p1 : {receive_one_message_func t1 l fd fd_state} @ fd_t")]]
-[[rc::tactics("by apply recvonemsg0.")]]
-[[rc::tactics("by apply recvonemsg1.")]]
-[[rc::tactics("by apply recvonemsg2.")]]
-[[rc::tactics("by apply recvonemsg3.")]]
-[[rc::tactics("by apply recvonemsg4.")]]
-[[rc::tactics("by apply recvonemsg5.")]]
+[[rc::requires("[curr_read_index t1]")]]
+[[rc::requires("[is_errno errno]")]]
+[[rc::exists( "n : Z")]]
+[[rc::returns("{if (bool_decide $ is_Some $ (packet_arrivals fd t1)) then 0 else -1} @ int<i32>")]]
+[[rc::ensures("[curr_read_index (t1 + 1)%nat]")]]
+[[rc::ensures("own p1 : {receive_one_message_func t1 fd fd_state} @ fd_t")]]
+[[rc::ensures("[is_errno n]")]]
+[[rc::ensures("{if (bool_decide $ is_Some $ (packet_arrivals fd t1)) then True else n = 80}")]]
+[[rc::tactics("all: destruct (packet_arrivals fd t1) eqn:E; try solve_goal.")]]
+[[rc::tactics("by apply packet_data_len.")]]
+[[rc::tactics("rewrite get_packet_data_no_pending => //=; eexists; solve_goal.")]]
+[[rc::tactics("by rewrite get_packet_data_no_pending.")]]
+[[rc::tactics("by rewrite receive_one_message_no_pending.")]]
+[[rc::tactics("by rewrite /add_pending_msg_to_scheduler E.")]]
 static
 int receive_one_message(struct fd_scheduler* fds, int fd) {
   /* NB: we really should use pre-allocated memory here to avoid page faults */
-  //struct message *msg = malloc(sizeof(*msg));
   struct message *msg = xmalloc(sizeof(*msg));
 
   /* we are not going to handle memory allocation failures */
@@ -136,7 +131,7 @@ int receive_one_message(struct fd_scheduler* fds, int fd) {
   /* receive data from FD */
   int n = read(fd, &msg->data, MAX_MESSAGE_LEN);
 
-  if (n <= 0) {
+  if (n < 0) {
     // FIXME: should handle closed FDs gracefully
     free(msg);
     return n;
@@ -147,32 +142,141 @@ int receive_one_message(struct fd_scheduler* fds, int fd) {
   }
 }
 
+// When the return value is non-negative it is a flag for whether we actually received a message otherwise it's an error flag (-1)
+[[rc::parameters("fd_state : fd_sched", "p1 : loc","fd : Z","t1 : nat", "errno : Z")]]
+[[rc::args("p1 @ &own<fd_state @ fd_t>", "fd @ int<i32>")]]
+[[rc::requires("[curr_read_index t1]")]]
+[[rc::requires("[is_errno errno]")]]
+[[rc::exists("m : nat", "flag : Z", "errno : Z")]]
+[[rc::returns("flag @ int<i32>")]]
+[[rc::ensures("[curr_read_index (t1 + (S m))]")]]
+[[rc::ensures("[is_errno errno]")]]
+[[rc::ensures("{fd_has_n_msgs fd m t1}")]]
+[[rc::ensures("{flag = bool_to_Z (bool_decide (m <> 0))%nat}")]]
+[[rc::ensures("own p1 : {receive_n_messages_func t1 fd fd_state (S m)} @ fd_t")]]
+[[rc::tactics("all: rewrite <- ?Nat.add_assoc, ?Nat.add_1_r; try apply simpl_fd_has_msgs_S; solve_goal.")]]
 static
 int receive_messages(struct fd_scheduler* fds, int fd) {
   int err;
+  int non_empty = 0;
+
+
+  [[rc::exists("i : nat", "err : Z", "flag : Z")]]
+  [[rc::exists("fd_state_mid : fd_sched", "n : Z")]]
+  [[rc::inv_vars("err : err @ int<i32>")]]
+  [[rc::inv_vars("fds : p1 @ &own<fd_state_mid @ fd_t>")]]
+  [[rc::inv_vars("non_empty : flag @ int<i32>")]]
+  [[rc::constraints("[curr_read_index (t1 +  (S i))]")]]
+  [[rc::constraints("{if (bool_decide $ is_Some $ (packet_arrivals fd (t1 +  i))) then err = 0"
+		    " else err = -1}")]]
+  [[rc::constraints("{ flag = if (decide (i = 0)%nat) then bool_to_Z (err =? 0) else 1}")]]
+  [[rc::constraints("{fd_state_mid = receive_n_messages_func t1 fd fd_state (S i)}")]]
+  [[rc::constraints("[is_errno n]")]]
+  [[rc::constraints("{if (bool_decide $ is_Some $ (packet_arrivals fd (t1 +   i))) then True else n = 80}")]]
+  [[rc::constraints("{fd_has_at_least_n_msgs fd i t1}")]]
   do {
     err = receive_one_message(fds, fd);
-  } while (!err);
+    if (!err) non_empty = 1;
+  }
+  while (!err);
 
   if (errno == EWOULDBLOCK || errno == EAGAIN)
     /* nothing else to receive for now, this is fine */
-    return 0;
+    return non_empty;
   else
     return err;
 }
 
-static
-int check_channels(struct fd_scheduler* fds) {
-  int err;
+
+// When the return value is non-negative it is a flag for whether we actually received a message otherwise it's an error flag (-1)
+//all messages received on all channels till time t have been read and added to the scheduler
+//calls recv messages on fd i for ni times
+[[rc::parameters("fd_state : fd_sched", "p1 : loc", "t1 : nat", "errno : Z")]]
+[[rc::args("p1 @ &own<fd_state @ fd_t>")]]
+[[rc::requires("[curr_read_index t1]")]]
+[[rc::requires("[is_errno errno]")]]
+[[rc::exists("ns : {list nat}", "flag : Z", "errno : Z")]]
+[[rc::returns("flag @ int<i32>")]]
+[[rc::ensures("[curr_read_index (t1 + num_reads_for_ns ns)%nat]")]]
+[[rc::ensures("[is_errno errno]")]]
+[[rc::ensures("{flag = bool_to_Z (bool_decide (Exists (λ n, (n <> 0)%nat) ns))}")]]
+[[rc::ensures("own p1 : {check_n_channels_func t1 fd_state (length (input_channels fd_state)) ns} @ fd_t")]]
+[[rc::ensures("{fds_have_n_msgs (input_channels fd_state) ns t1}")]]
+[[rc::tactics("all: simplify_channels; try solve_goal.")]]
+[[rc::tactics("rewrite Nat.add_1_r; erewrite take_S_r => //; apply fds_have_n_msgs_next_fd => //.")]]
+[[rc::tactics("apply Exists_app; right; apply Exists_cons_hd; solve_goal.")]]
+[[rc::tactics("rewrite receive_one_message_no_pending; by [ apply fd_has_n_msgs_implies_no_pending | rewrite -check_n_channels_S ].")]]
+[[rc::tactics("rewrite Nat.add_1_r; erewrite take_S_r => //; apply fds_have_n_msgs_next_fd => //.")]]
+[[rc::tactics("assert (¬ ((λ n, n <> 0) x')%nat) as HP by solve_goal; eapply Exists_last_false in HP; solve_goal.")]]
+[[rc::tactics("rewrite receive_one_message_no_pending; by [ apply fd_has_n_msgs_implies_no_pending | rewrite -check_n_channels_S ].")]]
+[[rc::tactics("repeat f_equal; lia.")]]
+[[rc::tactics("erewrite <- (take_ge (input_channels _)) => //; lia.")]]
+static int check_channels(struct fd_scheduler* fds) {
+  int fd, err, flag = 0;
+
+  [[rc::exists("i : nat", "errno : Z")]]
+  [[rc::exists("fd_state_mid : fd_sched")]]
+  [[rc::exists("ns : {list nat}", "flag : Z")]]
+  [[rc::inv_vars("ch : i @ int<u64>")]]
+  [[rc::inv_vars("fds : p1 @ &own<fd_state_mid @ fd_t>")]]
+  [[rc::inv_vars("flag : flag @ int<i32>")]]
+  [[rc::constraints("[curr_read_index (t1 + (num_reads_for_ns ns))]")]]
+  [[rc::constraints("[is_errno errno]")]]
+  [[rc::constraints("{fds_have_n_msgs (take i (input_channels fd_state)) ns t1}")]]
+  [[rc::constraints("{ flag = bool_to_Z (bool_decide (Exists (λ n, (n <> 0)%nat) ns))}")]]
+  [[rc::constraints("{fd_state_mid = check_n_channels_func t1 fd_state i ns}")]]
+  [[rc::constraints("{(0 ≤ i ≤ length (input_channels fd_state))%nat}")]]
   for (nfds_t ch = 0; ch < fds->num_channels; ch++) {
-      err = receive_messages(fds, fds->input_channels[ch]);
-      if (!err)
-        return err;
+    fd = fds->input_channels[ch];
+    err = receive_messages(fds, fd);
+    if (err < 0)
+      return err;
+    if (err > 0)
+      flag = 1;
   }
-  return 0;
+  return flag;
 }
 
-int fds_run(struct fd_scheduler* fds) {
+[[rc::parameters("fd_state : fd_sched", "p1 : loc", "t1 : nat", "errno : Z")]]
+[[rc::args("p1 @ &own<fd_state @ fd_t>")]]
+[[rc::requires("[curr_read_index t1]")]]
+[[rc::requires("[is_errno errno]")]]
+[[rc::exists("ns_list : {list (list nat)}")]]
+[[rc::returns("{0} @ int<i32>")]]
+[[rc::ensures("[curr_read_index (t1 + num_reads_for_ns_list ns_list)]")]]
+[[rc::ensures("own p1 : {check_channels_until_empty_func t1 fd_state ns_list} @ fd_t")]]
+[[rc::ensures("{fds_have_ns_list_msgs_done (input_channels fd_state) ns_list t1}")]]
+[[rc::tactics("all: simplify_channels; clear_cases; try solve_goal.")]]
+[[rc::tactics("2,3: destruct (bool_decide_reflect (err = 0)); first lia.")]]
+[[rc::tactics("case_bool_decide => //=; by apply fds_have_ns_list_msgs_done_base_run.")]]
+[[rc::tactics("case_bool_decide; by [ apply fds_have_ns_list_msgs_next_loop | apply fds_have_ns_list_msgs_done_next_run].")]]
+[[rc::tactics("by rewrite check_channels_until_empty_next.")]]
+int check_channels_until_empty(struct fd_scheduler* fds){
+  int err;
+
+  [[rc::exists("err : Z", "errno : Z")]]
+  [[rc::exists("fd_state_mid : fd_sched")]]
+  [[rc::exists("ns_list : {list (list nat)}", "flag : Z")]]
+  [[rc::inv_vars("err : err @ int<i32>")]]
+  [[rc::inv_vars("fds : p1 @ &own<fd_state_mid @ fd_t>")]]
+  [[rc::constraints("{0 <= err}")]]
+  [[rc::constraints("[curr_read_index (t1 + (num_reads_for_ns_list ns_list))]")]]
+  [[rc::constraints("[is_errno errno]")]]
+  [[rc::constraints("{if (bool_decide (err = 0)) then \
+											fds_have_ns_list_msgs_done (input_channels fd_state) ns_list t1 else \
+ 											fds_have_ns_list_msgs (input_channels fd_state) ns_list t1}")]]
+  [[rc::constraints("{fd_state_mid = check_channels_until_empty_func t1 fd_state ns_list}")]]
+  do {
+    err = check_channels(fds);
+    if (err < 0)
+      return err;
+  } while (err > 0);
+
+  return err;
+}
+
+// fds after one iteration will just be (npfp_dequeue (check_channels fds))
+int fds_run(struct fd_scheduler *fds) {
   int err;
 
   assert(fds->num_channels > 0);
@@ -180,9 +284,7 @@ int fds_run(struct fd_scheduler* fds) {
   while (1) {
     do {
       /* receive messages on all channels */
-      err = check_channels(fds);
-      if (err)
-        return err;
+      err = check_channels_until_empty(fds);
 
       /* get the highest-priority message */
       struct message *msg = npfp_dequeue(&fds->sched);
