examples/scheduler/src/proofs/fdsched/basic_definitions.v
@@ -1,90 +1,51 @@
 From refinedc.typing Require Export typing.
 From refinedc.examples.scheduler.src.fdsched Require Export axioms.
 
+Notation pdata := (list Z) (only parsing).
+
+Class PacketArrivals := {
+  packet_arrivals : FD → nat → option pdata
+}.
+
 Definition max_msg_len : Z :=
   (4096 - ly_size u8 - ly_size size_t - ly_size void* ).
 Global Opaque max_msg_len.
 
 Global Instance packet_ID_inhabited : Inhabited packet_ID :=
-  populate {|fd := inhabitant; arr_time := inhabitant; index := inhabitant|}.
-
-(** We parameterize the whole proof by a ground truth of arrivals *)
-Notation pdata := (list Z) (only parsing).
-Class PacketArrivals := {
-  packet_arrivals : nat → FD → list pdata
-}.
+  populate {|fd := inhabitant; read_index := inhabitant |}.
 
 Global Instance DecisionID : EqDecision packet_ID.
 Proof.
   solve_decision.
 Qed.
 
-Section EventLog.
+(* Since Cerberus sets the value of EWOULDBLOCK, we also define the value
+   of the errorcode EWOULDBLOCK to be [80]. *)
+(* Link to Cerberus definition : https://github.com/rems-project/cerberus/blob/84d9b28a6af7453e3591e353cf1de08963a2bb40/frontend/model/builtins.lem#L169 *)
+Definition EWOULDBLOCK : nat := 80.
+
+Section ReadIndex.
   Context `{typeG Σ}.
+  Global Instance curr_read_index_related_to A t :
+    RelatedTo (Σ := Σ) (λ x : A,curr_read_index (t x)) :=
+    {|rt_fic := FindDirect (λ t, curr_read_index t)%I |}.
 
-  Global Instance curr_log_related_to A l : RelatedTo (Σ := Σ) (λ x : A,curr_log (l x)) :=
-    {|rt_fic := FindDirect (λ l1, curr_log l1)%I |}.
-  Global Instance curr_time_related_to A t : RelatedTo (Σ := Σ) (λ x : A,curr_time (t x)) :=
-    {|rt_fic := FindDirect (λ t, curr_time t)%I |}.
-  Lemma subsume_curr_log B l l1 G :
-    (∃ x, ⌜l = l1 x⌝ ∗ G x)
-    ⊢ subsume (Σ := Σ) (curr_log l) (λ x : B, curr_log (l1 x)) G.
-  Proof. iIntros "(%x & -> & ?) Hcurr". iExists _. iFrame. Qed.
-  Definition subsume_curr_log_inst := [instance subsume_curr_log].
-  Global Existing Instance subsume_curr_log_inst.
-
-  Lemma subsume_curr_time B t t1 G:
+  Lemma subsume_curr_read_index B t t1 G:
     (∃ x, ⌜t = t1 x⌝ ∗ G x)
-    ⊢ subsume (Σ := Σ) (curr_time t) (λ x : B, curr_time (t1 x)) G.
+    ⊢ subsume (Σ := Σ) (curr_read_index t) (λ x : B, curr_read_index (t1 x)) G.
   Proof. iIntros "(%x & -> & ?) Hcurr". iExists _. iFrame. Qed.
-  Definition subsume_curr_time_inst := [instance subsume_curr_time].
-  Global Existing Instance subsume_curr_time_inst.
+  Definition subsume_curr_read_index_inst := [instance subsume_curr_read_index].
+  Global Existing Instance subsume_curr_read_index_inst.
 
-End EventLog.
-
-(** function to compute IDs of packets read so far *)
-Definition read_so_far_ID (l : list LogEntry) : list packet_ID :=
-  omap (λ e, if e is read_from_socket j _ then Some j else None) l.
+End ReadIndex.
 
 Section ReadSpecs.
   Context `{!PacketArrivals}.
 
-  (** Lookup in the arrival sequence using the ID. *)
   Definition get_packet_data (ID : packet_ID) : pdata :=
-    packet_arrivals (arr_time ID) (fd ID) !!! index ID.
+    take (Z.to_nat max_msg_len) (default inhabitant (packet_arrivals ID.(fd) ID.(read_index))).
 
-  (** function to compute data of a packet given its ID *)
-  Definition get_packet_data_option (ID : option packet_ID) : list Z:=
-    from_option get_packet_data inhabitant ID.
-
-  (** Get list of n packet IDs arriving at time t *)
-  Definition get_list_packets t (n : nat) (curr_fd : FD) : list packet_ID :=
-    (λ n, {|arr_time := t; index := n; fd := curr_fd|}) <$> seq 0 n.
-
-  (** list of packet ID's that have arrived at time [t] *)
-  Definition IDs_arrived_at  (t : nat) (fd : FD) : list packet_ID :=
-    let arrivals_at_t := packet_arrivals t fd in
-    let len := length arrivals_at_t in
-    get_list_packets t len fd.
-
-  (** Given a current time and a file descriptor generate all the packet IDs
-      that have arrived so far. *)
-  Definition IDs_arrived_upto (t : nat) (fd : FD) : list packet_ID :=
-    seq 0 t ≫= (λ n, IDs_arrived_at n fd ).
-
-  (** all the packet IDs that have arrived but not been read yet *)
-  Definition get_pending_packets_from_given_fd (t : nat) (l: list LogEntry) (fd : FD)
-    : list packet_ID :=
-    list_difference (IDs_arrived_upto t fd) (read_so_far_ID l).
-
-  (** get the ID of the head of pending packets list *)
-  Definition get_head_ID_option (t : nat) (l : list LogEntry) (fd : FD) : option packet_ID :=
-    head (get_pending_packets_from_given_fd t l fd).
-
-  (** get the ID of the head of pending packets list *)
-  Definition get_head_ID (t : nat) (l : list LogEntry) (fd : FD) : packet_ID :=
-    default inhabitant (get_head_ID_option t l fd).
+   Definition get_packet_data_option (ID : option packet_ID) : pdata:=
+     from_option get_packet_data inhabitant ID.
 
 End ReadSpecs.
-
-Global Opaque get_packet_data_option.
