examples/scheduler/src/proofs/fdsched/fdsched_extra.v
@@ -1,9 +1,52 @@
 From refinedc.examples.scheduler.src.fdsched Require Export message_extra.
 From refinedc.examples.scheduler.src.fdsched Require Export priority_extra.
 From refinedc.examples.scheduler.src.fdsched Require Export scheduler_extra.
-From refinedc.typing Require Export typing.
+From refinedc.examples.scheduler.src.fdsched Require Export misc_lemmas.
 From refinedc.examples.scheduler.src.fdsched Require Export basic_definitions.
 
+(** * upstream *)
+(* TODO: upstream the following definitions *)
+Global Instance simpl_plus_eq_l (x y z z' : nat):
+  SimplBothRel (=) (x + y + z)%nat (x + z')%nat (y + z = z')%nat.
+Proof. split; lia. Qed.
+
+Global Instance simpl_sum_list_cons l l' x :
+  SimplAndUnsafe (sum_list l + x = sum_list l')%nat (l' = l ++ [x]).
+Proof. intros ->; induction l => //=; lia. Qed.
+
+Global Instance simpl_add_0 m n :
+  SimplAndRel (=) n (n + m)%nat (m = 0)%nat.
+Proof. split; lia. Qed.
+
+Global Instance simpl_sum_list_nil l :
+  SimplAndRel (=) (sum_list l) 0%nat (∃ n, l = replicate n 0%nat).
+Proof.
+  split.
+  - intros [n ->]. rewrite sum_list_replicate; lia.
+  - induction l as [ | [ | ] l' IH] => /=; try lia.
+    + intros _. by exists 0%nat.
+    + intros.
+      destruct (IH ltac:(lia)) as [n ->].
+      exists (n + 1)%nat. by rewrite Nat.add_1_r.
+Qed.
+
+Global Instance simpl_list_trivial_match {A} (l : list A) :
+  SimplAnd (if l is [] then True else False) (l = []).
+Proof. split; solve_goal. Qed.
+
+Section upstream.
+  Context `{!typeG Σ}.
+
+  Lemma subsume_array_insert_id A l ly ty elts elts' i β G :
+    subsume (l ◁ₗ{β} array ly (<[ i := ty ]> elts)) (λ x : A, l ◁ₗ{β} array ly (elts' x)) G
+     where `{!CanSolve (elts !! i = Some ty)} :-
+      x ← (l ◁ₗ{β} array ly elts) :>> (λ x : A, l ◁ₗ{β} array ly (elts' x)); return G x.
+  Proof. move => ?. by rewrite list_insert_id. Qed.
+  Definition subsume_array_insert_id_inst := [instance subsume_array_insert_id].
+  Global Existing Instance subsume_array_insert_id_inst | 0.
+End upstream.
+
+(** * main definitions *)
 Record fd_sched := {
     input_channels : list FD;
     sched_state : npfp_sched;
@@ -42,21 +85,21 @@ Section RecieveOneMessageSpecification.
 
    (** Given a packet ID, generate the message corresponding to that packet ID *)
   Definition generate_msg_corresponding_to_packetID (id : packet_ID) : message_data :=
-    {|m_type := inhabitant; m_length := max_msg_len; m_id := id|}.
+    {| m_type := inhabitant; m_length := length (get_packet_data id); m_id := id|}.
 
   (** if pending packets is empty then add nothing to the scheduler else add
       the right message to the scheduler. *)
-  Definition add_pending_msg_to_scheduler (t :nat) (l1 : list LogEntry) (fd : FD) (sched_state : npfp_sched) : npfp_sched :=
-    let ID := (get_head_ID t l1 fd) in
-    let pending := get_pending_packets_from_given_fd t l1 fd in
-    if decide (pending = []) then sched_state else
+  Definition add_pending_msg_to_scheduler (t :nat)  (fd : FD) (sched_state : npfp_sched) : npfp_sched :=
+    let ID := {|fd := fd; read_index := t|} in
+    if (bool_decide (is_Some (packet_arrivals fd t))) then
       let msg := generate_msg_corresponding_to_packetID ID in
-      npfp_enqueue_func sched_state msg.
+      npfp_enqueue_func sched_state msg
+    else sched_state.
 
-  Definition receive_one_message_func (t :nat) (l : list LogEntry) (fd :FD) (fd_state : fd_sched) : fd_sched :=
+  Definition receive_one_message_func (t :nat) (fd :FD) (fd_state : fd_sched) : fd_sched :=
     {|
       input_channels := fd_state.(input_channels);
-      sched_state := add_pending_msg_to_scheduler t l fd fd_state.(sched_state);
+      sched_state := add_pending_msg_to_scheduler t fd fd_state.(sched_state);
     |}.
 
 End RecieveOneMessageSpecification.
@@ -69,136 +112,396 @@ Section RecieveOneMessageProof.
                     npfp_enqueue_func (sched_state fd_state) msg2) (msg1 = msg2) .
   Proof. by move => ->. Qed.
 
-  Global Instance simpl_and_get_packet_data_option_inst (n : packet_ID) t1 l fd
-    `{CanSolve (is_Some (get_head_ID_option t1 l fd))}
-    `{!IsEx n}:
-    SimplAndUnsafe
-      (get_packet_data_option (get_head_ID_option t1 l fd) `at_type` (int u8) ++
-         replicate (Z.to_nat max_msg_len -
-                      length (get_packet_data_option (get_head_ID_option t1 l fd)))
-         (uninit u8) =
-         get_packet_data  n `at_type` (int u8) ++
-           replicate (Z.to_nat max_msg_len - length (get_packet_data_option (Some n)))
-           (uninit u8))%I
-      (n = hd inhabitant (get_pending_packets_from_given_fd t1 l fd)).
+  Lemma packet_data_len pckt:
+    length (get_packet_data pckt) ≤ max_int i32.
   Proof.
-    rename select (CanSolve _) into HSome.
-    rewrite /CanSolve /get_head_ID_option in HSome.
-    move => ->.
-    case (get_pending_packets_from_given_fd t1 l fd) eqn: EQ; first by contradict HSome.
-    by rewrite /get_head_ID_option EQ //=.
+    rewrite /get_packet_data take_length.
+    unfold_opaque max_msg_len; solve_goal.
   Qed.
 
-  Global Instance simpl_and_message_equality msg1 msg2 :
-    SimplAnd (msg1 = msg2)
-      (msg1.(m_type) = msg2.(m_type)
-       ∧ msg1.(m_length) = msg2.(m_length)
-       ∧ msg1.(m_id) = msg2.(m_id)).
-  Proof. destruct msg1, msg2. split; naive_solver. Qed.
-
-  Lemma recvonemsg0 t1 l fd:
-    (if bool_decide (is_Some (get_head_ID_option t1 l fd)) then max_msg_len else -1) ≤ 0 →
-    ∃ n' : nat,
-      (get_packet_data_option (get_head_ID_option t1 l fd) `at_type` (int u8))%I =
-        replicate n' (uninit u8)
-      ∧ replicate (Z.to_nat max_msg_len - length (get_packet_data_option (get_head_ID_option t1 l fd)))
-          (uninit u8) =
-          replicate
-            (length (get_packet_data_option (get_head_ID_option t1 l fd)) +
-               (Z.to_nat max_msg_len - length (get_packet_data_option (get_head_ID_option t1 l fd))) - n')
-            (uninit u8)
-      ∧ (n' <=
-           length (get_packet_data_option (get_head_ID_option t1 l fd)) +
-             (Z.to_nat max_msg_len - length (get_packet_data_option (get_head_ID_option t1 l fd))))%nat.
+  Lemma receive_one_message_no_pending t fd fd_state :
+    packet_arrivals fd t = None →
+    receive_one_message_func t fd fd_state = fd_state.
   Proof.
-    exists 0%nat; split.
-    * unfold_opaque @get_packet_data_option.
-      have Hfalse: (¬ is_Some (get_head_ID_option t1 l fd)) by solve_goal.
-      rewrite -eq_None_not_Some in Hfalse.
-      by rewrite Hfalse.
-    * split; try solve_goal.
-      have Hfalse: (¬ is_Some (get_head_ID_option t1 l fd)) by solve_goal.
-      rewrite -eq_None_not_Some in Hfalse.
-      rewrite Hfalse. unfold_opaque @get_packet_data_option.
-      simpl.
-      solve_goal.
+    rewrite /receive_one_message_func /add_pending_msg_to_scheduler => ->.
+    by destruct fd_state.
   Qed.
 
-  Lemma recvonemsg1 t1 l fd:
-     (if bool_decide (is_Some (get_head_ID_option t1 l fd)) then max_msg_len else -1) ≤ 0 →
-     (ly_size u8 * 4079)%nat =
-  (ly_size u8 *
-   (length (get_packet_data_option (get_head_ID_option t1 l fd)) +
-      (Z.to_nat max_msg_len - length (get_packet_data_option (get_head_ID_option t1 l fd)))))%nat.
-  Proof.
-    move => ?.
-    have Hfalse: (¬ is_Some (get_head_ID_option t1 l fd)) by solve_goal.
-    rewrite -eq_None_not_Some in Hfalse.
-    rewrite !Hfalse. unfold_opaque @get_packet_data_option.
-    simpl.
-    solve_goal.
-    Qed.
-
-  Lemma recvonemsg2 t1 l fd :
-    (if bool_decide (is_Some (get_head_ID_option t1 l fd)) then max_msg_len else -1) ≤ 0 →
-    (if bool_decide (is_Some (get_head_ID_option t1 l fd)) then max_msg_len else -1) =
-      (if decide (get_pending_packets_from_given_fd t1 l fd = []) then -1 else 0).
-  Proof.
-    move => ?.
-    rewrite /get_head_ID_option.
-    case (get_pending_packets_from_given_fd t1 l fd) eqn:EQ; first by done.
-    have Hfalse: bool_decide (is_Some (get_head_ID_option t1 l fd)) = false by solve_goal.
-    by rewrite /get_head_ID bool_decide_eq_false -eq_None_not_Some head_None EQ in Hfalse.
-  Qed.
-
-  Lemma recvonemsg3 t1 l fd fd_state :
-    (if bool_decide (is_Some (get_head_ID_option t1 l fd)) then max_msg_len else -1) ≤ 0 →
-    fd_state = receive_one_message_func t1 l fd fd_state.
-  Proof.
-    move => ?.
-    have Hfalse: bool_decide (is_Some (get_head_ID_option t1 l fd)) = false by solve_goal.
-    rewrite /get_head_ID bool_decide_eq_false -eq_None_not_Some head_None in Hfalse.
-    rewrite /receive_one_message_func /add_pending_msg_to_scheduler !Hfalse //=.
-    destruct fd_state; f_equiv; done.
-  Qed.
-
-  Lemma recvonemsg4 t1 l fd :
-    ¬ (if bool_decide (is_Some (get_head_ID_option t1 l fd)) then max_msg_len else -1) ≤ 0 →
-    0 = (if decide (get_pending_packets_from_given_fd t1 l fd = []) then -1 else 0).
-  Proof.
-    move => ?.
-    have Htrue: bool_decide (is_Some (get_head_ID_option t1 l fd)) = true by solve_goal.
-    rewrite /get_head_ID_option bool_decide_eq_true in Htrue.
-    rewrite decide_bool_decide.
-    case (bool_decide (get_pending_packets_from_given_fd t1 l fd = [])) eqn: EQ; try done.
-    rewrite bool_decide_eq_true in EQ.
-    rewrite EQ in Htrue.
-    by contradict Htrue.
-  Qed.
-
-  Lemma recvonemsg5 t1 l fd fd_state:
-    ¬ (if bool_decide (is_Some (get_head_ID_option t1 l fd)) then max_msg_len else -1) ≤ 0 →
-    npfp_enqueue_func (sched_state fd_state)
-                      {|
-                        m_type :=
-                          message_identify_type_coq
-                            (hd inhabitant (get_pending_packets_from_given_fd t1 l fd));
-                        m_length := if bool_decide (is_Some (get_head_ID_option t1 l fd))
-                                    then max_msg_len else -1;
-                        m_id := hd inhabitant (get_pending_packets_from_given_fd t1 l fd)
-                      |}
-    = add_pending_msg_to_scheduler t1 l fd (sched_state fd_state).
-  Proof.
-    move => ?.
-    have Htrue: bool_decide (is_Some (get_head_ID_option t1 l fd)) = true by solve_goal.
-    rewrite  /add_pending_msg_to_scheduler !Htrue //= decide_bool_decide.
-    rewrite bool_decide_eq_true /get_head_ID_option in Htrue.
-    have ->: bool_decide (get_pending_packets_from_given_fd t1 l fd = []) = false
-        by rewrite bool_decide_eq_false -head_is_Some.
-    rewrite /get_priority /npfp_enqueue_func.
-    case (get_pending_packets_from_given_fd t1 l fd) eqn:EQ; first by contradict Htrue.
-    f_equiv; rewrite /hd; last by rewrite /get_head_ID /get_head_ID_option EQ //=.
-    by rewrite /generate_msg_corresponding_to_packetID /get_head_ID /get_head_ID_option EQ //= max_msg_len_simpl.
-  Qed.
+  Lemma get_packet_data_no_pending fd t :
+    packet_arrivals fd t = None →
+    get_packet_data {| fd := fd; read_index := t |} = [].
+  Proof. rewrite /get_packet_data => /= ->; solve_goal. Qed.
 
 End RecieveOneMessageProof.
+
+Section ReceiveMessagesSpecs.
+
+  Context `{!PacketArrivals}.
+
+  Fixpoint receive_n_messages_func (t : nat) (fd : FD) (fd_state :fd_sched) (n : nat) : fd_sched :=
+    match n with
+    | 0%nat => fd_state
+    | S n' => let new_fd_state := receive_n_messages_func t fd fd_state n' in
+              receive_one_message_func (t + n') fd new_fd_state
+    end.
+
+  Definition fd_has_at_least_n_msgs (fd : FD) (m : nat) (init : nat) : Prop :=
+      ∀ i, (0 ≤ i < m)%nat -> is_Some (packet_arrivals fd (init + i)%nat).
+
+  Definition fd_has_n_msgs (fd : FD) (m : nat) (init : nat) : Prop :=
+    fd_has_at_least_n_msgs fd m init ∧
+      ¬ is_Some (packet_arrivals fd (init + m)).
+
+End ReceiveMessagesSpecs.
+
+#[export] Hint Unfold add_pending_msg_to_scheduler receive_one_message_func : core.
+
+Section RecieveMessagesProof.
+
+  Context `{!PacketArrivals}.
+
+  Lemma simpl_fd_has_msgs_0 (fd : FD) (init : nat) :
+    fd_has_at_least_n_msgs fd 0 init.
+  Proof. rewrite /fd_has_at_least_n_msgs; lia. Qed.
+
+  Lemma simpl_fd_has_msgs_S (fd : FD) (i init : nat) :
+    (fd_has_at_least_n_msgs fd i init ∧ is_Some (packet_arrivals fd (init + i)%nat)) → (fd_has_at_least_n_msgs fd (S i) init).
+  Proof.
+    intros [H1 H2].
+    unfold fd_has_at_least_n_msgs.
+    intros j.
+    intros [Hlb Hub].
+    destruct (decide (j = i)) as [-> | Hneq] => //.
+    + apply H1; lia.
+  Qed.
+
+End RecieveMessagesProof.
+
+#[export] Hint Resolve simpl_fd_has_msgs_0 simpl_fd_has_msgs_S : core.
+
+Section CheckChannelsSpec.
+
+  Context `{!PacketArrivals}.
+
+  Fixpoint check_n_channels_func' (t : nat)  (fd_state : fd_sched) (fds : list Z) (ns : list nat) : fd_sched :=
+    match fds, ns with
+    | [], [] => fd_state
+    | fd :: fds', n :: ns' =>
+        let fd_state' := receive_n_messages_func t fd fd_state n in
+        check_n_channels_func' (t + n + 1)%nat fd_state' fds' ns'
+    | _, _ => fd_state
+    end.
+
+  Definition check_n_channels_func (t : nat) (fd_state : fd_sched) (n : nat)  (ns : list nat) :=
+    let fds := take n (input_channels fd_state) in
+    check_n_channels_func' t fd_state fds ns.
+
+  (** `ns` is the number of messages on each fd; `init` is the initial read index *)
+  Fixpoint fds_have_n_msgs (fds : list FD) (ns : list nat) (init : nat) : Prop :=
+    match fds, ns with
+    | [], [] => True
+    | fd :: fds, n :: ns =>
+        (* Since the code will execute an additional empty read, the next read index
+           needs to be incremented by the number of messages read + 1 (empty read) *)
+        fd_has_n_msgs fd n init ∧ fds_have_n_msgs fds ns (init + n + 1)%nat
+    | _, _ => False
+    end.
+
+  (** Computes the number of calls made to read given that ns is a list of
+      of number of read messages for each fd. Since the code reads until it
+      hits an empty read, we need to add 1 for each fd; hence the `length ns` *)
+  Definition num_reads_for_ns (ns : list nat) := (length ns + sum_list ns)%nat.
+
+End CheckChannelsSpec.
+
+Section CheckChannelsProofs.
+
+  Context `{!PacketArrivals} `{!typeG Σ}.
+
+  Lemma fds_have_n_msgs_next_fd fds fd ns n init :
+    fds_have_n_msgs fds ns init →
+    fd_has_n_msgs fd n (init + num_reads_for_ns ns) →
+    fds_have_n_msgs (fds ++ [fd]) (ns ++ [n]) init.
+  Proof.
+    induction fds as [ | fd' fds IH] in ns, init |- *.
+    - destruct ns => //=. by rewrite Nat.add_0_r.
+    - intros Hfds Hfd.
+      destruct ns as [ | n' ns] => //. split; first naive_solver.
+      apply IH; first naive_solver.
+      eapply eq_ind_r => //.
+      rewrite /num_reads_for_ns => /=; lia.
+  Qed.
+
+  Global Instance simpl_num_reads_for_ns_nil ns :
+    SimplAndRel (=) (num_reads_for_ns ns) 0%nat (ns = []).
+  Proof. split; by [subst | destruct ns]. Qed.
+
+  Global Instance simpl_num_reads_for_ns_cons ns ns' n :
+    SimplAndUnsafe (num_reads_for_ns ns + (S n) = num_reads_for_ns ns')%nat
+      (ns' = ns ++ [n]).
+  Proof.
+    move => ->. rewrite /num_reads_for_ns => //=.
+    rewrite sum_list_with_app app_length => /=. lia.
+  Qed.
+
+
+  Lemma receive_n_messages_input_channels init fd fd_state n :
+    input_channels (receive_n_messages_func init fd fd_state n) =
+      input_channels fd_state.
+  Proof. induction n in fd_state, init |- * => //=. Qed.
+
+  Lemma check_channels_input_channels' init fd_state fds ns :
+    input_channels (check_n_channels_func' init fd_state fds ns) =
+      input_channels fd_state.
+  Proof.
+    induction fds in init, fd_state, ns |- *.
+    - simpl. by destruct ns.
+    - simpl. destruct ns => //.
+      rewrite IHfds.
+      by rewrite receive_n_messages_input_channels.
+  Qed.
+
+  Lemma check_channels_input_channels init fd_state n ns :
+    input_channels (check_n_channels_func init fd_state n ns) =
+      input_channels fd_state.
+  Proof.
+    rewrite /check_n_channels_func.
+    by rewrite check_channels_input_channels'.
+  Qed.
+
+  Lemma fd_has_n_msgs_implies_no_pending fd n init :
+    fd_has_n_msgs fd n init →
+    packet_arrivals fd (init + n)%nat = None.
+  Proof.
+    move  => [_ Hnone].
+    by apply eq_None_not_Some.
+  Qed.
+
+  Lemma check_n_channels_S' init fd_state n fds fd ns :
+    length ns = length fds →
+    check_n_channels_func' init fd_state (fds ++ [fd]) (ns ++ [n]) =
+      receive_n_messages_func (init + num_reads_for_ns ns) fd (check_n_channels_func' init fd_state fds ns) n.
+  Proof.
+    induction fds in n, fd, init, fd_state, ns |- *.
+    - destruct ns => //= _.
+      rewrite (proj1 (simpl_num_reads_for_ns_nil [])); f_equal; lia.
+    - destruct ns as [ | n' ns'] => //= Hlen.
+      rewrite IHfds; last lia.
+      f_equal.
+      unfold_opaque num_reads_for_ns => /=; lia.
+  Qed.
+
+  Lemma fds_have_n_msgs_same_len fds ns init :
+    fds_have_n_msgs fds ns init →
+    length ns = length fds.
+  Proof.
+    induction fds in ns, init |- *.
+    - by destruct ns.
+    - destruct ns => //=.
+      by intros [_ ->%IHfds].
+  Qed.
+
+  Lemma check_n_channels_S i init fd_state n fd ns :
+    fds_have_n_msgs (take i (input_channels fd_state)) ns init →
+    input_channels fd_state !! i = Some fd →
+    check_n_channels_func init fd_state (i + 1)%nat (ns ++ [n]) =
+      receive_n_messages_func (init + num_reads_for_ns ns) fd (check_n_channels_func init fd_state i ns) n.
+  Proof.
+    intros ?%fds_have_n_msgs_same_len ?.
+    rewrite /check_n_channels_func .
+    rewrite Nat.add_1_r.
+    erewrite take_S_r => //.
+    rewrite check_n_channels_S' => //.
+  Qed.
+
+  Lemma Exists_last_false {A} P l (x : A) :
+    ¬ (P x) →
+    Exists P l ↔ Exists P (l ++ [x]).
+  Proof.
+    intros HPx. split => HP.
+    - apply Exists_app; by left.
+    - apply Exists_app in HP as [ | [ | ?%Exists_nil]%Exists_inv] => //.
+  Qed.
+
+End CheckChannelsProofs.
+
+Global Opaque num_reads_for_ns.
+
+Section CheckUntilEmptySpecs.
+
+  Context `{!PacketArrivals}.
+
+  Fixpoint check_channels_until_empty_func (t : nat) (fd_state : fd_sched) (ns_list : list (list nat)) : fd_sched :=
+    match ns_list with
+    | [] => fd_state
+    | ns :: ns_list' =>
+        let fd_state' := check_n_channels_func t fd_state (length (input_channels fd_state)) ns in
+        check_channels_until_empty_func (t + num_reads_for_ns ns) fd_state' ns_list'
+    end.
+
+  Definition num_reads_for_ns_list (ns : list (list nat)) : nat :=
+    (sum_list (map num_reads_for_ns ns))%nat.
+
+  (* ns_list has the number of read messages on each descriptor (ns) for every call to check_channels *)
+  (* this predicate assumes that all the calls to check_channels didn't fail - i.e. there was one successful read on some descriptor. check the definition below for the failed case *)
+  Fixpoint fds_have_ns_list_msgs (fds : list FD) (ns_list : list (list nat)) (init : nat) : Prop :=
+    match ns_list with
+    | [] => True
+    | ns :: ns_list' => Exists (λ n, (n <> 0)%nat) ns ∧ (* this holds because of the assumption that check_channels hasn't failed yet *)
+                        fds_have_n_msgs fds ns init ∧
+                        fds_have_ns_list_msgs fds ns_list' (init + num_reads_for_ns ns)
+    end.
+
+  (* there will be as many "ns" as the # of calls to `check_channels` *)
+  (* this predicate assumes that the last call to `check_channels` failed to find any msgs *)
+  (* assuming that `check_channes` was called at least once *)
+  Definition fds_have_ns_list_msgs_done (fds : list FD) (ns_list : list (list nat)) (init : nat) : Prop :=
+    let ns_list' := (take (length ns_list - 1)%nat ns_list) in
+    fds_have_ns_list_msgs fds ns_list' init ∧
+    match last ns_list with
+    | None => False (* it should never be None *)
+    | Some ns => fds_have_n_msgs fds ns (init + num_reads_for_ns_list ns_list')%nat ∧ Forall (λ n, (n = 0)%nat) ns
+    end.
+
+End CheckUntilEmptySpecs.
+
+Section CheckUntilEmptyProofs.
+
+  Context `{!PacketArrivals}.
+
+  Lemma num_reads_for_ns_list_nil :
+    num_reads_for_ns_list [] = 0%nat.
+  Proof. done. Qed.
+
+  Lemma num_reads_for_ns_list_cons ns ns_list :
+    num_reads_for_ns_list (ns :: ns_list) = (num_reads_for_ns ns + num_reads_for_ns_list ns_list)%nat.
+  Proof. done. Qed.
+
+  (* Hint Rewrite @num_reads_for_ns_list_nil @num_reads_for_ns_list_cons. *)
+
+  Global Instance simpl_and_rel_num_reads_init (t : nat) (ns : list nat) (ns_list : list (list nat)) :
+    SimplAndUnsafe (t + num_reads_for_ns ns = t + num_reads_for_ns_list ns_list)%nat (ns_list = [ns]).
+  Proof. intros ->. auto. Qed.
+
+  Global Instance simpl_and_rel_num_reads_cons (ns : list nat) (ns_list ns_list' : list (list nat)) :
+    SimplAndUnsafe (num_reads_for_ns_list ns_list + num_reads_for_ns ns = num_reads_for_ns_list ns_list')%nat (ns_list' = ns_list ++ [ns]).
+  Proof.
+    intros ->. rewrite /num_reads_for_ns_list => /=.
+    rewrite map_app; simpl; rewrite sum_list_with_app => /=; lia.
+  Qed.
+
+  Lemma check_channels_until_empty_input_channels init fd_state ns_list :
+    input_channels (check_channels_until_empty_func init fd_state ns_list) =
+      input_channels fd_state.
+  Proof.
+    induction ns_list as [ | ???IH] in init, fd_state |- * => //=.
+    rewrite IH.
+    by rewrite check_channels_input_channels.
+  Qed.
+
+  Lemma fds_have_ns_list_msgs_next_loop fds ns_list ns init :
+    fds_have_ns_list_msgs fds ns_list init →
+    fds_have_n_msgs fds ns (init + num_reads_for_ns_list ns_list) →
+    Exists (λ n : nat, n ≠ 0%nat) ns →
+    fds_have_ns_list_msgs fds (ns_list ++ [ns]) init.
+  Proof.
+    induction ns_list as [ | ns' ns_list' IHns ] in init |- *.
+    - simpl. rewrite /num_reads_for_ns_list Nat.add_0_r => /= _?? //.
+    - simpl. intros [Hnon_empty_ns' [Hns' Hns_list']].
+      rewrite /num_reads_for_ns_list => /=.
+      intros Hns Hnon_empty_ns.
+      split => //.
+      split => //.
+      apply IHns => //.
+      rewrite /num_reads_for_ns_list. by rewrite -Nat.add_assoc.
+  Qed.
+
+  Lemma check_channels_until_empty_next init fd_state ns ns_list :
+    fds_have_ns_list_msgs (input_channels fd_state) ns_list init →
+    fds_have_n_msgs (input_channels fd_state) ns (init + num_reads_for_ns_list ns_list) →
+    check_channels_until_empty_func init fd_state (ns_list ++ [ns]) =
+      check_n_channels_func (init + num_reads_for_ns_list ns_list) (check_channels_until_empty_func init fd_state ns_list) (length (input_channels fd_state)) ns.
+  Proof.
+    induction ns_list as [ | ns' ns_list' IHns ] in init,fd_state |- *.
+    - rewrite /num_reads_for_ns_list => /= ??; f_equal; lia.
+    - intros Hns_list Hns.
+      rewrite -app_comm_cons.
+      cbn [check_channels_until_empty_func].
+      rewrite IHns.
+      all: rewrite ?check_channels_input_channels ?check_channels_until_empty_input_channels.
+      + f_equal; first by rewrite -Nat.add_assoc.
+      + naive_solver.
+      + rewrite /num_reads_for_ns_list in Hns. simpl in Hns.
+        by rewrite -Nat.add_assoc.
+  Qed.
+
+  Lemma fds_have_ns_list_msgs_done_base_run (ns : list nat) fd_state init:
+    ¬ Exists (λ n : nat, n ≠ 0%nat) ns →
+    fds_have_n_msgs (input_channels fd_state) ns init →
+    fds_have_ns_list_msgs_done (input_channels fd_state) [ns] init.
+  Proof.
+    intros ??. split => //. rewrite last_singleton => /=.
+    split.
+    - by rewrite num_reads_for_ns_list_nil Nat.add_0_r.
+    - apply not_Exists_Forall in H0; last solve_decision.
+      eapply Forall_impl => // x /=; lia.
+  Qed.
+
+  Lemma fds_have_ns_list_msgs_done_next_run (ns : list nat) ns_list fd_state init:
+    ¬ Exists (λ n : nat, n ≠ 0%nat) ns →
+    fds_have_ns_list_msgs (input_channels fd_state) ns_list init →
+    fds_have_n_msgs (input_channels fd_state) ns (init + num_reads_for_ns_list ns_list) →
+    fds_have_ns_list_msgs_done (input_channels fd_state) (ns_list ++ [ns]) init.
+  Proof.
+    intros ???. split => //.
+    { rewrite take_app_length' => //. rewrite app_length => /=; lia. }
+    rewrite last_snoc. split.
+    - rewrite take_app_length' => //. rewrite app_length => /=; lia.
+    - apply not_Exists_Forall in H0; last solve_decision.
+      eapply Forall_impl => // x /=; lia.
+  Qed.
+
+End CheckUntilEmptyProofs.
+
+Ltac simplify_channels :=
+  repeat
+    match goal with
+    | Hchannels : context G [input_channels (check_n_channels_func _ _ _ _)] |- _ =>
+        rewrite check_channels_input_channels in Hchannels
+    | Hchannels : context G [input_channels (check_channels_until_empty_func _ _ _)] |- _ => rewrite check_channels_until_empty_input_channels in Hchannels end;
+  rewrite ?check_channels_input_channels ?check_channels_until_empty_input_channels.
+
+Ltac clear_cases :=
+  repeat match goal with
+         | H : ?T |- _ =>
+           (* Keep current location and case distinction info. *)
+           lazymatch T with
+           | CURRENT_LOCATION _ _ => idtac
+           | CASE_DISTINCTION_INFO _ _ => idtac
+           | _ => fail
+           end;
+           clear H
+         end.
+
+Section error_num.
+
+  Context `{!typeG Σ}.
+
+  Definition FindErrNo :=
+    {| fic_A := Z; fic_Prop n := @is_errno Σ n; |}.
+  Lemma find_in_context_err_no `{!typeG Σ} T:
+    (∃ n, is_errno n ∗ T n) ⊢ find_in_context (FindErrNo) T.
+  Proof. iIntros "(% & H)". iExists n. by iFrame. Qed.
+  Definition find_in_context_err_no_inst :=
+    [instance find_in_context_err_no with FICSyntactic].
+  Global Existing Instance find_in_context_err_no_inst | 1.
+  Global Instance related_to_err_no A n' : RelatedTo (λ x : A, is_errno (n' x)) := {| rt_fic := FindErrNo |}.
+
+  Lemma subsume_is_errno A n n' G :
+    subsume (@is_errno Σ n) (λ x : A, is_errno (n' x)) G :-
+      ∃ x, exhale ⌜ n = n' x⌝; return (G x).
+  Proof. iIntros "(%x & -> & ?) ?". iExists x. iFrame. Qed.
+  Definition subsume_is_errno_inst := [instance subsume_is_errno].
+  Global Existing Instance subsume_is_errno_inst.
+
+End error_num.
