examples/scheduler/src/proofs/fdsched/axioms.v
@@ -3,30 +3,25 @@ From refinedc.typing Require Export typing.
 (** Wrapper type for file descriptors *)
 Notation FD := Z (only parsing).
 
-(** the ID for a packet is given by a tuple of fd, time and index in the arrivals at that time *)
+(** The id for a packet is given by a tuple of the FD on which it arrives and the
+    value of [read_index] when it is read by the program. *)
 Record packet_ID := PACKET_ID {
   fd : FD;
-  arr_time : nat;
-  index : nat;
+  read_index : nat;
 }.
 
-(** The data type for interesting events we record in the log*)
-Inductive LogEntry :=
-| read_from_socket (j : packet_ID) (t : nat)
-| callback_dispatched (j : packet_ID) (t : nat)
-| callback_returned (j : packet_ID) (t : nat).
-
-Section EventLog.
+Section ReadIndex.
   Context `{typeG Σ}.
 
-  Axiom curr_time : nat → iProp Σ.
-  Axiom curr_log : list LogEntry → iProp Σ.
+  Axiom curr_read_index : nat → iProp Σ.
+  Axiom is_errno : Z → iProp Σ.
 
-End EventLog.
+End ReadIndex.
 
-(** function to look up the type of the message *)
+
 Notation num_msg_types := (max_int u8 + 1) (only parsing).
 
+(** function to look up the type of the message *)
 Axiom message_identify_type_coq : packet_ID → nat.
 
 Axiom msg_type_bounded : ∀ msg, message_identify_type_coq msg < num_msg_types.
