examples/scheduler/src/proofs/fdsched/misc_lemmas.v
@@ -1,0 +1,55 @@
+From stdpp Require Import list.
+From stdpp Require Import sets.
+From Coq Require Export ssreflect.
+
+  (* upstream to stdpp? *)
+Lemma list_difference_app_r `{!EqDecision A} (l k k' : list A) :
+  list_difference l (k ++ k') =
+    list_difference (list_difference l k) k'.
+Proof.
+  induction l in k,k' |- * => //=.
+  case_decide.
+  - case_decide => /=; first by rewrite IHl.
+    case_decide; [ by rewrite IHl | set_solver ].
+  - case_decide => /=; first set_solver.
+    case_decide => /=; first set_solver.
+    by rewrite IHl.
+Qed.
+
+(* upstream or factor into a separate library lemma *)
+Lemma unique_elems_cons_2 {A} (p p' : A) ps :
+  NoDup (p :: p' :: ps) →
+  NoDup (p :: ps).
+Proof.
+  move => Hunique /=. constructor.
+  - by apply NoDup_cons in Hunique as [[? ?]%not_elem_of_cons ?].
+  - by apply NoDup_cons in Hunique as [? [? ?]%NoDup_cons].
+Qed.
+
+(* upstream or factor into a separate library lemma *)
+Lemma list_difference_unique_elems `{! EqDecision A} (p : A) ps :
+  NoDup (p :: ps) → list_difference ps [p] = ps.
+Proof.
+  induction ps in p |- * => Hunique //=. case_decide.
+  - apply NoDup_cons in Hunique as [[Hp _]%not_elem_of_cons _].
+    set_solver.
+  - rewrite IHps => //. by eapply (unique_elems_cons_2 _ a).
+Qed.
+
+Lemma drop_lt {A} (l : list A) n:
+  (drop n l <> []) → (n < length l)%nat.
+Proof.
+  induction n in l|-*.
+  - destruct l => //=; lia.
+  - destruct l => //= ?.
+    apply -> Nat.succ_lt_mono. by apply IHn.
+Qed.
+
+Lemma drop_ge'{A} (l : list A) n:
+  (drop n l = []) → (length l ≤ n)%nat.
+Proof.
+  induction n in l|-*.
+  - destruct l => //=; lia.
+  - destruct l => //= ?; first lia.
+    apply le_n_S. by apply IHn.
+Qed.
